theories/vm/Semantics.v
@@ -1,12 +1,26 @@
 From Books Require Import Tactics.
-From Books.vm Require Import Syntax.
-From Stdlib Require Import List NArith.
+From Books.vm Require Export Syntax.
+From Stdlib Require Import List NArith Lia.
 Import ListNotations.
 Open Scope N_scope.
 
-Definition list_update {X : Type} (l : list X) (idx : N) (x : X) : list X :=
-  if idx =? N.of_nat (length l) then x :: l else
-  rev (snd (fold_left (fun '(idx', a) i => (idx' + 1, (if idx =? idx' then x else i) :: a)) l (0, []))).
+Fixpoint repeat {A : Type} (x : A) (n : nat) : list A :=
+  match n with
+  | O => []
+  | S n' => x :: repeat x n'
+  end.
+
+Definition list_update {X : Type} (default : X) (l : list X) (idx : N) (x : X) : list X :=
+  let len := N.of_nat (length l) in
+  let idx_nat := N.to_nat idx in
+  let l' :=
+    if len <=? idx then
+      (* extend with default to the left so the target index exists *)
+      repeat default (N.to_nat (idx - len) + 1) ++ l
+    else l in
+  let len' := length l' in
+  let pos_from_left := (len' - 1 - idx_nat)%nat in
+  firstn pos_from_left l' ++ [x] ++ skipn (S pos_from_left) l'.
 
 Inductive step (p : program) : stack -> pc -> stack -> pc -> Prop :=
 | SConst : forall n st pc,
@@ -23,7 +37,7 @@ Inductive step (p : program) : stack -> pc -> stack -> pc -> Prop :=
     step p (n2 :: n1 :: st) pc (n1 - n2 :: st) (pc + 1)
 | SDup : forall idx n st pc,
     p pc = Some Dup ->
-    nth_error st (length st - N.to_nat idx) = Some n ->
+    nth_error st (length st - N.to_nat idx - 1) = Some n ->
     step p (idx :: st) pc (n :: st) (pc + 1)
 | SSwap : forall n1 n2 st pc,
     p pc = Some Swap ->
@@ -33,7 +47,7 @@ Inductive step (p : program) : stack -> pc -> stack -> pc -> Prop :=
     step p st pc (N.of_nat (length st) :: st) (pc + 1)
 | SStore : forall idx n st pc,
     p pc = Some Store ->
-    step p (n :: idx :: st) pc (list_update st (N.of_nat (length st) - idx) n) (pc + 1)
+    step p (n :: idx :: st) pc (list_update 0 st (N.of_nat (length st) - idx) n) (pc + 1)
 | SJmp : forall pc' st pc,
     p pc = Some (Jmp pc') ->
     step p st pc st pc'
@@ -44,8 +58,19 @@ Inductive step (p : program) : stack -> pc -> stack -> pc -> Prop :=
 | SJnzF : forall pc' st pc,
     p pc = Some (Jnz pc') ->
     step p (0 :: st) pc (0 :: st) (pc + 1).
-
 Hint Constructors step : core.
+
+Inductive exec_prog (p : program) : stack -> pc -> stack -> pc -> Prop :=
+| ExecDone : forall st pc,
+    p pc = None ->
+    exec_prog p st pc st pc
+| ExecStep : forall st1 st2 pc1 pc2 st3 pc3,
+    p pc1 <> None ->
+    (* One step of execution *)
+    step p st1 pc1 st2 pc2 ->
+    (* Continue executing *)
+    exec_prog p st2 pc2 st3 pc3 ->
+    exec_prog p st1 pc1 st3 pc3.
 
 Ltac solve_ppc :=
   match goal with
@@ -64,4 +89,27 @@ Proof.
   destruct H1 as (I & PPCI). revert st1' pc1' st2' pc2' p pc st PPCI H H0.
   destruct I; intros.
   all: inv H; solve_ppc; inv H0; solve_ppc; try easy.
+Qed.
+
+Theorem exec_prog_deterministic :
+  forall p st pc st1' pc1' st2' pc2',
+    exec_prog p st pc st1' pc1' ->
+    exec_prog p st pc st2' pc2' ->
+    st1' = st2' /\ pc1' = pc2'.
+Proof.
+  intros. induction H.
+  - (* Terminated *) inv H0. easy. contradiction.
+  - (* Continue *) inv H0. contradiction. clear H3.
+      pose proof (step_deterministic _ _ _ _ _ _ _ H1 H4). destruct H0; subst.
+      apply IHexec_prog. assumption.
+Qed.
+
+Lemma exec_prog_no_step :
+  forall p st pc st1 pc1,
+    exec_prog p st pc st1 pc1 ->
+    ~ exists st1' pc1', step p st1 pc1 st1' pc1'.
+Proof.
+  intros. induction H.
+  - intro. destruct H0 as (st' & pc' & Step). inv Step; rewrite H in H0; inv H0.
+  - apply IHexec_prog.
 Qed.
