theories/Tactics.v
@@ -1,1 +1,17 @@
+From Stdlib Require Import NArith Lia ZifyN ZifyBool List.
+Import ListNotations.
+Open Scope N_scope.
+
 Ltac inv H := inversion H; subst; clear H.
+
+Ltac eqb_false :=
+  match goal with [|- context[?x =? ?y]] => replace (x =? y) with false by lia end.
+Ltac eqb_true :=
+  match goal with [|- context[?x =? ?y]] => replace (x =? y) with true by lia end.
+Ltac eqb_hammer := repeat (eqb_false || eqb_true).
+
+Ltac solve_in :=
+  repeat match goal with
+  | [H: In _ [] |- _ ] => inv H
+  | [H: In ?op _ |- _] => inv H; [easy|]
+  end.
