theories/compiler/AEVAL_proofs.v
@@ -1,0 +1,179 @@
+From Books Require Import compiler.Compiler vm.Semantics lang.Semantics Tactics.
+From Stdlib Require Import List Lia Nat.
+Import ListNotations.
+
+Definition N_of_storeval (s : storeval) : N :=
+  match s with
+  | Nat n => n
+  | Bool b => if b then 1 else 0
+  end.
+
+Definition mem_models_store (l : layout) (st : stack) (s : store) :=
+  forall i v,
+    s i = Some v <-> 
+      (exists idx, l i = Some idx /\
+       nth_error st (length st - N.to_nat idx - 1) = Some (N_of_storeval v)).
+
+Lemma nth_error_some_idx_valid :
+  forall {A} (l : list A) i v,
+    nth_error l i = Some v ->
+    (i < length l)%nat.
+Proof.
+  induction l; intros.
+  - rewrite nth_error_nil in H. inv H.
+  - rewrite nth_error_cons in H. destruct i. inv H. simpl. lia.
+      simpl. apply Arith_base.lt_n_S_stt. eauto.
+Qed.
+
+Lemma fold_left_cons :
+  forall {A B} f (h : A) t (i : B),
+    fold_left f (h :: t) i = fold_left f t (f i h).
+Proof. reflexivity. Qed.
+
+Lemma program_of_plist_exact :
+  forall t pc h,
+    program_of_plist pc (h :: t) pc = Some h.
+Admitted.
+
+Lemma exec_prog_cons :
+  forall h t st pc st' pc' st'' pc'',
+    vm.Semantics.step (program_of_plist pc [h]) st pc st' pc' ->
+    exec_prog (program_of_plist pc (h :: t)) st' pc' st'' pc'' ->
+    exec_prog (program_of_plist pc (h :: t)) st pc st'' pc''.
+Proof.
+  intros. unfold program_of_plist in H. simpl in H.
+  inv H; rewrite N.eqb_refl in H1; inv H1.
+  all: try solve [econstructor; [
+      now rewrite program_of_plist_exact
+    | constructor; (apply program_of_plist_exact || eassumption)
+    | assumption]].
+  econstructor.
+    now rewrite program_of_plist_exact.
+    eapply SJnzF. apply program_of_plist_exact. assumption.
+Qed.
+
+(* Lemma step_trans :
+  forall l1 l2 st pc st' pc' st'' pc'',
+    vm.Semantics.step (program_of_plist pc l1) st pc st' pc' ->
+    vm.Semantics.step (program_of_plist pc (l1 ++ l2)) st pc st'' pc''.
+Proof.
+  induction l1; intros.
+  - unfold program_of_plist in H; simpl in H. inv H; inv H0.
+  - simpl. inv H; rewrite program_of_plist_exact in H0; inv H0. *)
+
+Lemma exec_prog_trans :
+  forall l1 l2 st pc st' pc' st'' pc'',
+    exec_prog (program_of_plist pc l1) st pc st' pc' ->
+    exec_prog (program_of_plist pc' l2) st' pc' st'' pc'' ->
+    exec_prog (program_of_plist pc (l1 ++ l2)) st pc st'' pc''.
+Admitted.
+
+Lemma models_store_cons :
+  forall l st s h,
+    mem_models_store l st s ->
+    mem_models_store l (h :: st) s.
+Admitted.
+(* Proof.
+  induction l; intros.
+  - unfold mem_models_store. intros. specialize (H i v). destruct H.
+    split; intro.
+    -- specialize (H H1). destruct H as (idx & Eq & Lt & Err). eexists. split. eassumption.
+       split. simpl length. rewrite Nat2N.inj_succ, <- N.add_1_r. lia.
+       simpl length. rewrite <- PeanoNat.Nat.sub_add_distr, PeanoNat.Nat.add_comm. simpl.
+       replace (Datatypes.length st - N.to_nat idx)%nat with (S (Datatypes.length st - N.to_nat idx - 1)).
+       rewrite nth_error_cons_succ. apply Err.
+       rewrite <- PeanoNat.Nat.sub_add_distr, PeanoNat.Nat.add_comm. simpl.
+       rewrite <- PeanoNat.Nat.sub_succ_l, PeanoNat.Nat.sub_succ. reflexivity. lia.
+    -- destruct H1 as (idx & Eq & Lt & Err). apply H0. exists idx. split. assumption.
+       split. simpl length in Lt. rewrite Nat2N.inj_succ, <- N.add_1_r in Lt.
+       destruct (N.eq_dec idx (N.of_nat (length st))). subst idx.
+       rewrite Nat2N.id in Err. simpl length in Err.
+       rewrite <- PeanoNat.Nat.sub_add_distr, PeanoNat.Nat.add_comm in Err. simpl in Err.
+       rewrite PeanoNat.Nat.sub_diag in Err. simpl in Err. inv Err. *)
+
+Lemma of_nat_length_LN : forall {A} (l : list A),
+  N.of_nat (length l) = LN l.
+Proof. reflexivity. Qed.
+
+Lemma LN_app : forall {A} (l1 l2 : list A),
+  LN l1 + LN l2 = LN (l1 ++ l2).
+Proof.
+  induction l1; intros.
+  - reflexivity.
+  - unfold LN in *. simpl length. repeat rewrite Nat2N.inj_succ. rewrite <- IHl1. lia.
+Qed.
+
+Lemma LN_app_cons : forall {A} (l : list A) (x : A),
+  LN (l ++ [x]) = LN l + 1.
+Proof.
+  intros. rewrite <- LN_app. reflexivity.
+Qed.
+
+Theorem AEVAL_correct :
+  forall a l s n pc st,
+    mem_models_store l st s ->
+    aeval s a n ->
+    exec_prog (program_of_plist pc (AEVAL pc l a))
+      st pc 
+      (n :: st) (pc + N.of_nat (length (AEVAL pc l a))).
+Proof.
+  induction a; intros.
+  - (* ConstNat *) unfold program_of_plist; simpl.
+        econstructor.
+          rewrite N.eqb_refl. discriminate.
+          constructor. now rewrite N.eqb_refl.
+          inv H0.
+            constructor. now eqb_hammer.
+            solve_in.
+  - (* VarNat *)
+    unfold program_of_plist; simpl; unfold LOAD.
+    destruct (l i) eqn:E; simpl.
+    -- econstructor.
+         eqb_hammer. discriminate.
+         constructor. now eqb_hammer.
+         inv H0.
+           econstructor.
+             now eqb_hammer. {
+             apply SDup. now eqb_hammer.
+             specialize (H i (Nat n)). rewrite E, H3 in H. destruct H as (L & R).
+             specialize (L ltac:(eauto)).
+             destruct st.
+              exfalso. destruct L, H. rewrite nth_error_nil in H0. inv H0.
+              apply nth_error_nth'. rewrite length_cons. lia.
+           } { replace (pc + 1 + 1) with (pc + 2) by lia.
+             specialize (H i (Nat n)). rewrite E, H3 in H. destruct H. specialize (H eq_refl).
+             replace (nth _ st _) with n. constructor.
+             now eqb_hammer.
+             destruct H as (idx & Eq & Err). inv Eq.
+             eapply nth_error_nth in Err. now rewrite Err.
+           } solve_in.
+    -- inv H0. specialize (H i (Nat n)). destruct H. specialize (H H3). destruct H as (idx & Eq & Err).
+       rewrite E in Eq. discriminate. solve_in.
+  - (* Plus *)
+    simpl AEVAL. inv H0. replace op with Plus in * by solve_in. inv H1.
+      eapply exec_prog_trans. eauto.
+      eapply exec_prog_trans. eapply IHa2. apply models_store_cons. eassumption. eassumption.
+      econstructor. now rewrite program_of_plist_exact.
+      constructor; now rewrite program_of_plist_exact.
+      simpl in H6. inv H6. repeat rewrite of_nat_length_LN.
+      repeat rewrite <- LN_app. change (LN [Syntax.Plus]) with 1.
+      repeat rewrite <- N.add_assoc. rewrite LN_app. apply ExecDone.
+      unfold program_of_plist. simpl. replace (_ =? _) with false. reflexivity.
+      rewrite <- LN_app. lia.
+  - (* Minus *)
+    simpl AEVAL. inv H0. replace op with Minus in * by solve_in. inv H1.
+      eapply exec_prog_trans. eauto.
+      eapply exec_prog_trans. eapply IHa2. apply models_store_cons. eassumption. eassumption.
+      econstructor. now rewrite program_of_plist_exact.
+      constructor; now rewrite program_of_plist_exact.
+      simpl in H6. inv H6. repeat rewrite of_nat_length_LN.
+      repeat rewrite <- LN_app. change (LN [Syntax.Minus]) with 1.
+      repeat rewrite <- N.add_assoc. rewrite LN_app. apply ExecDone.
+      unfold program_of_plist. simpl. replace (_ =? _) with false. reflexivity.
+      rewrite <- LN_app. lia.
+  - (* Mult *)
+    simpl AEVAL. inv H0. replace op with Mult in * by solve_in. inv H1.
+      eapply exec_prog_trans. eauto.
+      eapply exec_prog_trans. eapply IHa2. apply models_store_cons. eassumption. eassumption.
+      econstructor. (* oh my *)
+Admitted.
