theories/compiler/Layout.v
@@ -1,3 +1,6 @@
 From Books Require Import lang.Syntax.
 
-Definition var_layout : Type := ident -> N.
+Definition layout : Type := ident -> option N.
+
+Definition layout_of_alist (l : list (ident * N)) : layout :=
+  List.fold_left (fun a '(i, addr) => update ieqb a i (Some addr)) l (fun _ => None).
